feat: use typeclass for protocol invariants

src/DY.Core.Bytes.fst
@@ -31,7 +31,8 @@ let rec length b =
   | Hash msg ->
     32
 
-noeq type crypto_usages = {
+class crypto_usages = {
+   [@@@FStar.Tactics.Typeclasses.no_method]
   __nothing: unit;
 }
 
@@ -41,23 +42,23 @@ let default_crypto_usages = {
 }
 
 [@@"opaque_to_smt"]
-val get_usage: crypto_usages -> bytes -> GTot usage
-let get_usage cusages b =
+val get_usage: {|crypto_usages|} -> bytes -> GTot usage
+let get_usage #cusages b =
   match b with
   | Rand usg label len time ->
     usg
   | _ -> Unknown
 
 [@@"opaque_to_smt"]
-val get_label: crypto_usages -> bytes -> GTot label
-let rec get_label cusages b =
+val get_label: {|crypto_usages|} -> bytes -> GTot label
+let rec get_label #cusages b =
   match b with
   | Literal buf ->
     public
   | Rand usg label len time ->
     label
   | Concat left right ->
-    meet (get_label cusages left) (get_label cusages right)
+    meet (get_label left) (get_label right)
   | Aead key nonce msg ad ->
     public
   | Pk sk ->
@@ -67,62 +68,62 @@ let rec get_label cusages b =
   | Vk sk ->
     public
   | Sign sk nonce msg ->
-    get_label cusages msg
+    get_label msg
   | Hash msg ->
-    get_label cusages msg
+    get_label msg
 
 [@@"opaque_to_smt"]
-val get_sk_label: crypto_usages -> bytes -> GTot label
-let get_sk_label cusages pk =
+val get_sk_label: {|crypto_usages|} -> bytes -> GTot label
+let get_sk_label #cusages pk =
   match pk with
-  | Pk sk -> get_label cusages sk
+  | Pk sk -> get_label sk
   | _ -> public
 
 [@@"opaque_to_smt"]
-val get_sk_usage: crypto_usages -> bytes -> GTot usage
-let get_sk_usage cusages pk =
+val get_sk_usage: {|crypto_usages|} -> bytes -> GTot usage
+let get_sk_usage #cusages pk =
   match pk with
-  | Pk sk -> get_usage cusages sk
+  | Pk sk -> get_usage sk
   | _ -> Unknown
 
 [@@"opaque_to_smt"]
-val get_signkey_label: crypto_usages -> bytes -> GTot label
-let get_signkey_label cusages pk =
+val get_signkey_label: {|crypto_usages|} -> bytes -> GTot label
+let get_signkey_label #cusages pk =
   match pk with
-  | Vk sk -> get_label cusages sk
+  | Vk sk -> get_label sk
   | _ -> public
 
 [@@"opaque_to_smt"]
-val get_signkey_usage: crypto_usages -> bytes -> GTot usage
-let get_signkey_usage cusages pk =
+val get_signkey_usage: {|crypto_usages|} -> bytes -> GTot usage
+let get_signkey_usage #cusages pk =
   match pk with
-  | Vk sk -> get_usage cusages sk
+  | Vk sk -> get_usage sk
   | _ -> Unknown
 
 noeq
 type crypto_predicates (cusages:crypto_usages) = {
-  aead_pred: tr:trace -> key:bytes{AeadKey? (get_usage cusages key)} -> nonce:bytes -> msg:bytes -> ad:bytes -> prop;
+  aead_pred: tr:trace -> key:bytes{AeadKey? (get_usage key)} -> nonce:bytes -> msg:bytes -> ad:bytes -> prop;
   aead_pred_later:
     tr1:trace -> tr2:trace ->
-    key:bytes{AeadKey? (get_usage cusages key)} -> nonce:bytes -> msg:bytes -> ad:bytes ->
+    key:bytes{AeadKey? (get_usage key)} -> nonce:bytes -> msg:bytes -> ad:bytes ->
     Lemma
     (requires aead_pred tr1 key nonce msg ad /\ tr1 <$ tr2)
     (ensures aead_pred tr2 key nonce msg ad)
   ;
 
-  pkenc_pred: tr:trace -> pk:bytes{PkdecKey? (get_sk_usage cusages pk)} -> msg:bytes -> prop;
+  pkenc_pred: tr:trace -> pk:bytes{PkdecKey? (get_sk_usage pk)} -> msg:bytes -> prop;
   pkenc_pred_later:
     tr1:trace -> tr2:trace ->
-    pk:bytes{PkdecKey? (get_sk_usage cusages pk)} -> msg:bytes ->
+    pk:bytes{PkdecKey? (get_sk_usage pk)} -> msg:bytes ->
     Lemma
     (requires pkenc_pred tr1 pk msg /\ tr1 <$ tr2)
     (ensures pkenc_pred tr2 pk msg)
   ;
 
-  sign_pred: tr:trace -> vk:bytes{SigKey? (get_signkey_usage cusages vk)} -> msg:bytes -> prop;
+  sign_pred: tr:trace -> vk:bytes{SigKey? (get_signkey_usage vk)} -> msg:bytes -> prop;
   sign_pred_later:
     tr1:trace -> tr2:trace ->
-    vk:bytes{SigKey? (get_signkey_usage cusages vk)} -> msg:bytes ->
+    vk:bytes{SigKey? (get_signkey_usage vk)} -> msg:bytes ->
     Lemma
     (requires sign_pred tr1 vk msg /\ tr1 <$ tr2)
     (ensures sign_pred tr2 vk msg)
@@ -145,162 +146,171 @@ let default_crypto_predicates cusages = {
   sign_pred_later = (fun tr1 tr2 vk msg -> ());
 }
 
-noeq type crypto_invariants = {
+class crypto_invariants = {
+  [@@@FStar.Tactics.Typeclasses.tcinstance]
   usages: crypto_usages;
+  [@@@FStar.Tactics.Typeclasses.no_method]
   preds: crypto_predicates usages;
 }
 
+let aead_pred {|cinvs:crypto_invariants|} = cinvs.preds.aead_pred
+let aead_pred_later {|cinvs:crypto_invariants|} = cinvs.preds.aead_pred_later
+let pkenc_pred {|cinvs:crypto_invariants|} = cinvs.preds.pkenc_pred
+let pkenc_pred_later {|cinvs:crypto_invariants|} = cinvs.preds.pkenc_pred_later
+let sign_pred {|cinvs:crypto_invariants|} = cinvs.preds.sign_pred
+let sign_pred_later {|cinvs:crypto_invariants|} = cinvs.preds.sign_pred_later
+
 [@@"opaque_to_smt"]
-val bytes_invariant: crypto_invariants -> trace -> bytes -> prop
-let rec bytes_invariant cinvs tr b =
+val bytes_invariant: {|crypto_invariants|} -> trace -> bytes -> prop
+let rec bytes_invariant #cinvs tr b =
   match b with
   | Literal buf ->
     True
   | Rand usage label len time ->
     event_at tr time (RandGen usage label len)
   | Concat left right ->
-    bytes_invariant cinvs tr left /\
-    bytes_invariant cinvs tr right
+    bytes_invariant tr left /\
+    bytes_invariant tr right
   | Aead key nonce msg ad ->
-    bytes_invariant cinvs tr key /\
-    bytes_invariant cinvs tr nonce /\
-    bytes_invariant cinvs tr msg /\
-    bytes_invariant cinvs tr ad /\
-    (get_label cinvs.usages nonce) `can_flow tr` public /\
-    (get_label cinvs.usages ad) `can_flow tr` public /\
+    bytes_invariant tr key /\
+    bytes_invariant tr nonce /\
+    bytes_invariant tr msg /\
+    bytes_invariant tr ad /\
+    (get_label nonce) `can_flow tr` public /\
+    (get_label ad) `can_flow tr` public /\
     (
       (
         // Honest case
-        AeadKey? (get_usage cinvs.usages key) /\
+        AeadKey? (get_usage key) /\
         cinvs.preds.aead_pred tr key nonce msg ad /\
-        (get_label cinvs.usages msg) `can_flow tr` (get_label cinvs.usages key)
+        (get_label msg) `can_flow tr` (get_label key)
       ) \/ (
         // Attacker case
-        (get_label cinvs.usages key) `can_flow tr` public /\
-        (get_label cinvs.usages msg) `can_flow tr` public
+        (get_label key) `can_flow tr` public /\
+        (get_label msg) `can_flow tr` public
       )
     )
   | Pk sk ->
-    bytes_invariant cinvs tr sk
+    bytes_invariant tr sk
   | PkEnc pk nonce msg ->
-    bytes_invariant cinvs tr pk /\
-    bytes_invariant cinvs tr nonce /\
-    bytes_invariant cinvs tr msg /\
+    bytes_invariant tr pk /\
+    bytes_invariant tr nonce /\
+    bytes_invariant tr msg /\
     (
       (
         // Honest case
-        PkdecKey? (get_sk_usage cinvs.usages pk) /\
-        (get_label cinvs.usages msg) `can_flow tr` (get_sk_label cinvs.usages pk) /\
-        (get_label cinvs.usages msg) `can_flow tr` (get_label cinvs.usages nonce) /\
+        PkdecKey? (get_sk_usage pk) /\
+        (get_label msg) `can_flow tr` (get_sk_label pk) /\
+        (get_label msg) `can_flow tr` (get_label nonce) /\
         cinvs.preds.pkenc_pred tr pk msg
       ) \/ (
         // Attacker case
-        (get_label cinvs.usages pk) `can_flow tr` public /\
-        (get_label cinvs.usages nonce) `can_flow tr` public /\
-        (get_label cinvs.usages msg) `can_flow tr` public
+        (get_label pk) `can_flow tr` public /\
+        (get_label nonce) `can_flow tr` public /\
+        (get_label msg) `can_flow tr` public
       )
     )
   | Vk sk ->
-    bytes_invariant cinvs tr sk
+    bytes_invariant tr sk
   | Sign sk nonce msg ->
-    bytes_invariant cinvs tr sk /\
-    bytes_invariant cinvs tr nonce /\
-    bytes_invariant cinvs tr msg /\
+    bytes_invariant tr sk /\
+    bytes_invariant tr nonce /\
+    bytes_invariant tr msg /\
     (
       (
         // Honest case
-        SigKey? (get_signkey_usage cinvs.usages (Vk sk)) /\
+        SigKey? (get_signkey_usage (Vk sk)) /\
         cinvs.preds.sign_pred tr (Vk sk) msg
       ) \/ (
         // Attacker case
-        (get_label cinvs.usages sk) `can_flow tr` public /\
-        (get_label cinvs.usages nonce) `can_flow tr` public /\
-        (get_label cinvs.usages msg) `can_flow tr` public
+        (get_label sk) `can_flow tr` public /\
+        (get_label nonce) `can_flow tr` public /\
+        (get_label msg) `can_flow tr` public
       )
     )
   | Hash msg ->
-    bytes_invariant cinvs tr msg
+    bytes_invariant tr msg
 
 val bytes_invariant_later:
-  cinvs:crypto_invariants ->
+  {|crypto_invariants|} ->
   tr1:trace -> tr2:trace -> msg:bytes ->
   Lemma
-  (requires bytes_invariant cinvs tr1 msg /\ tr1 <$ tr2)
-  (ensures bytes_invariant cinvs tr2 msg)
-  [SMTPat (bytes_invariant cinvs tr1 msg); SMTPat (tr1 <$ tr2)]
-let rec bytes_invariant_later cinvs tr1 tr2 msg =
+  (requires bytes_invariant tr1 msg /\ tr1 <$ tr2)
+  (ensures bytes_invariant tr2 msg)
+  [SMTPat (bytes_invariant tr1 msg); SMTPat (tr1 <$ tr2)]
+let rec bytes_invariant_later #cinvs tr1 tr2 msg =
   normalize_term_spec bytes_invariant;
   match msg with
   | Literal buf -> ()
   | Rand usage label len time -> ()
   | Concat left right ->
-    bytes_invariant_later cinvs tr1 tr2 left;
-    bytes_invariant_later cinvs tr1 tr2 right
+    bytes_invariant_later tr1 tr2 left;
+    bytes_invariant_later tr1 tr2 right
   | Aead key nonce msg ad -> (
-    bytes_invariant_later cinvs tr1 tr2 key;
-    bytes_invariant_later cinvs tr1 tr2 nonce;
-    bytes_invariant_later cinvs tr1 tr2 msg;
-    bytes_invariant_later cinvs tr1 tr2 ad;
-    match get_usage cinvs.usages key with
+    bytes_invariant_later tr1 tr2 key;
+    bytes_invariant_later tr1 tr2 nonce;
+    bytes_invariant_later tr1 tr2 msg;
+    bytes_invariant_later tr1 tr2 ad;
+    match get_usage key with
     | AeadKey _ -> FStar.Classical.move_requires (cinvs.preds.aead_pred_later tr1 tr2 key nonce msg) ad
     | _ -> ()
   )
   | Pk sk ->
-    bytes_invariant_later cinvs tr1 tr2 sk
+    bytes_invariant_later tr1 tr2 sk
   | PkEnc pk nonce msg -> (
-    bytes_invariant_later cinvs tr1 tr2 pk;
-    bytes_invariant_later cinvs tr1 tr2 nonce;
-    bytes_invariant_later cinvs tr1 tr2 msg;
-    match get_sk_usage cinvs.usages pk with
+    bytes_invariant_later tr1 tr2 pk;
+    bytes_invariant_later tr1 tr2 nonce;
+    bytes_invariant_later tr1 tr2 msg;
+    match get_sk_usage pk with
     | PkdecKey _ -> FStar.Classical.move_requires (cinvs.preds.pkenc_pred_later tr1 tr2 pk) msg
     | _ -> ()
   )
   | Vk sk ->
-    bytes_invariant_later cinvs tr1 tr2 sk
+    bytes_invariant_later tr1 tr2 sk
   | Sign sk nonce msg -> (
-    bytes_invariant_later cinvs tr1 tr2 sk;
-    bytes_invariant_later cinvs tr1 tr2 nonce;
-    bytes_invariant_later cinvs tr1 tr2 msg;
-    match get_signkey_usage cinvs.usages (Vk sk) with
+    bytes_invariant_later tr1 tr2 sk;
+    bytes_invariant_later tr1 tr2 nonce;
+    bytes_invariant_later tr1 tr2 msg;
+    match get_signkey_usage (Vk sk) with
     | SigKey _ -> FStar.Classical.move_requires (cinvs.preds.sign_pred_later tr1 tr2 (Vk sk)) msg
     | _ -> ()
   )
   | Hash msg ->
-    bytes_invariant_later cinvs tr1 tr2 msg
+    bytes_invariant_later tr1 tr2 msg
 
 (*** Various predicates ***)
 
-val is_knowable_by: crypto_invariants -> label -> trace -> bytes -> prop
-let is_knowable_by cinvs lab tr b =
-  bytes_invariant cinvs tr b /\ (get_label cinvs.usages b) `can_flow tr` lab
+val is_knowable_by: {|crypto_invariants|} -> label -> trace -> bytes -> prop
+let is_knowable_by #cinvs lab tr b =
+  bytes_invariant tr b /\ (get_label b) `can_flow tr` lab
 
-val is_publishable: crypto_invariants -> trace -> bytes -> prop
-let is_publishable cinvs tr b =
-  is_knowable_by cinvs public tr b
+val is_publishable: {|crypto_invariants|} -> trace -> bytes -> prop
+let is_publishable #cinvs tr b =
+  is_knowable_by public tr b
 
-val is_secret: crypto_invariants -> label -> trace -> bytes -> prop
-let is_secret cinvs lab tr b =
-  bytes_invariant cinvs tr b /\ (get_label cinvs.usages b) == lab
+val is_secret: {|crypto_invariants|} -> label -> trace -> bytes -> prop
+let is_secret #cinvs lab tr b =
+  bytes_invariant tr b /\ (get_label b) == lab
 
-val is_verification_key: crypto_invariants -> string -> label -> trace -> bytes -> prop
-let is_verification_key cinvs usg lab tr b =
-  is_publishable cinvs tr b /\ (get_signkey_label cinvs.usages b) == lab /\
-  get_signkey_usage cinvs.usages b == SigKey usg
+val is_verification_key: {|crypto_invariants|} -> string -> label -> trace -> bytes -> prop
+let is_verification_key #cinvs usg lab tr b =
+  is_publishable tr b /\ (get_signkey_label b) == lab /\
+  get_signkey_usage b == SigKey usg
 
-val is_signature_key: crypto_invariants -> string -> label -> trace -> bytes -> prop
-let is_signature_key cinvs usg lab tr b =
-  is_secret cinvs lab tr b /\
-  get_usage cinvs.usages b == SigKey usg
+val is_signature_key: {|crypto_invariants|} -> string -> label -> trace -> bytes -> prop
+let is_signature_key #cinvs usg lab tr b =
+  is_secret lab tr b /\
+  get_usage b == SigKey usg
 
-val is_encryption_key: crypto_invariants -> string -> label -> trace -> bytes -> prop
-let is_encryption_key cinvs usg lab tr b =
-  is_publishable cinvs tr b /\ (get_sk_label cinvs.usages b) == lab /\
-  get_sk_usage cinvs.usages b == PkdecKey usg
+val is_encryption_key: {|crypto_invariants|} -> string -> label -> trace -> bytes -> prop
+let is_encryption_key #cinvs usg lab tr b =
+  is_publishable tr b /\ (get_sk_label b) == lab /\
+  get_sk_usage b == PkdecKey usg
 
-val is_decryption_key: crypto_invariants -> string -> label -> trace -> bytes -> prop
-let is_decryption_key cinvs usg lab tr b =
-  is_secret cinvs lab tr b /\
-  get_usage cinvs.usages b == PkdecKey usg
+val is_decryption_key: {|crypto_invariants|} -> string -> label -> trace -> bytes -> prop
+let is_decryption_key #cinvs usg lab tr b =
+  is_secret lab tr b /\
+  get_usage b == PkdecKey usg
 
 (*** Literal ***)
 
@@ -327,11 +337,11 @@ let literal_to_bytes_to_literal lit =
 
 // Lemma for attacker knowledge theorem
 val literal_to_bytes_is_publishable:
-  cinvs:crypto_invariants -> tr:trace ->
+  {|crypto_invariants|} -> tr:trace ->
   lit:FStar.Seq.seq FStar.UInt8.t ->
   Lemma
-  (is_publishable cinvs tr (literal_to_bytes lit))
-let literal_to_bytes_is_publishable cinvs tr lit =
+  (is_publishable tr (literal_to_bytes lit))
+let literal_to_bytes_is_publishable #cinvs tr lit =
   normalize_term_spec literal_to_bytes;
   normalize_term_spec bytes_invariant;
   normalize_term_spec get_label
@@ -357,12 +367,12 @@ let length_literal_to_bytes lit =
   normalize_term_spec length
 
 val bytes_invariant_literal_to_bytes:
-  cinvs:crypto_invariants -> tr:trace ->
+  {|crypto_invariants|} -> tr:trace ->
   lit:FStar.Seq.seq FStar.UInt8.t ->
   Lemma
-  (ensures bytes_invariant cinvs tr (literal_to_bytes lit))
-  [SMTPat (bytes_invariant cinvs tr (literal_to_bytes lit))]
-let bytes_invariant_literal_to_bytes cinvs tr lit =
+  (ensures bytes_invariant tr (literal_to_bytes lit))
+  [SMTPat (bytes_invariant tr (literal_to_bytes lit))]
+let bytes_invariant_literal_to_bytes #cinvs tr lit =
   normalize_term_spec literal_to_bytes;
   normalize_term_spec bytes_invariant
 
@@ -395,28 +405,28 @@ let split_concat left right =
 
 // Lemma for attacker knowledge theorem
 val concat_preserves_publishability:
-  cinvs:crypto_invariants -> tr:trace ->
+  {|crypto_invariants|} -> tr:trace ->
   b1:bytes -> b2:bytes ->
   Lemma
-  (requires is_publishable cinvs tr b1 /\ is_publishable cinvs tr b2)
-  (ensures is_publishable cinvs tr (concat b1 b2))
-let concat_preserves_publishability cinvs tr b1 b2 =
+  (requires is_publishable tr b1 /\ is_publishable tr b2)
+  (ensures is_publishable tr (concat b1 b2))
+let concat_preserves_publishability #cinvs tr b1 b2 =
   normalize_term_spec concat;
   normalize_term_spec bytes_invariant;
   normalize_term_spec get_label
 
 // Lemma for attacker knowledge theorem
 val split_preserves_publishability:
-  cinvs:crypto_invariants -> tr:trace ->
+  {|crypto_invariants|} -> tr:trace ->
   b:bytes -> i:nat ->
   Lemma
-  (requires is_publishable cinvs tr b)
+  (requires is_publishable tr b)
   (ensures (
     match split b i with
     | None -> True
-    | Some (b1, b2) -> is_publishable cinvs tr b1 /\ is_publishable cinvs tr b2
+    | Some (b1, b2) -> is_publishable tr b1 /\ is_publishable tr b2
   ))
-let split_preserves_publishability cinvs tr b i =
+let split_preserves_publishability #cinvs tr b i =
   normalize_term_spec split;
   normalize_term_spec bytes_invariant;
   normalize_term_spec get_label
@@ -453,64 +463,64 @@ let split_length b i =
   normalize_term_spec length
 
 val bytes_invariant_concat:
-  cinvs:crypto_invariants -> tr:trace ->
+  {|crypto_invariants|} -> tr:trace ->
   b1:bytes -> b2:bytes ->
   Lemma
-  (requires bytes_invariant cinvs tr b1 /\ bytes_invariant cinvs tr b2)
-  (ensures bytes_invariant cinvs tr (concat b1 b2))
-  [SMTPat (bytes_invariant cinvs tr (concat b1 b2))]
-let bytes_invariant_concat cinvs tr b1 b2 =
+  (requires bytes_invariant tr b1 /\ bytes_invariant tr b2)
+  (ensures bytes_invariant tr (concat b1 b2))
+  [SMTPat (bytes_invariant tr (concat b1 b2))]
+let bytes_invariant_concat #cinvs tr b1 b2 =
   normalize_term_spec concat;
   normalize_term_spec bytes_invariant
 
 val bytes_invariant_split:
-  cinvs:crypto_invariants -> tr:trace ->
+  {|crypto_invariants|} -> tr:trace ->
   b:bytes -> i:nat ->
   Lemma
-  (requires bytes_invariant cinvs tr b)
+  (requires bytes_invariant tr b)
   (ensures (
     match split b i with
     | None -> True
-    | Some (b1, b2) -> bytes_invariant cinvs tr b1 /\ bytes_invariant cinvs tr b2
+    | Some (b1, b2) -> bytes_invariant tr b1 /\ bytes_invariant tr b2
   ))
-  [SMTPat (bytes_invariant cinvs tr b); SMTPat (split b i)]
-let bytes_invariant_split cinvs tr b i =
+  [SMTPat (bytes_invariant tr b); SMTPat (split b i)]
+let bytes_invariant_split #cinvs tr b i =
   normalize_term_spec split;
   normalize_term_spec bytes_invariant
 
 val get_label_concat:
-  cusages:crypto_usages ->
+  {|crypto_usages|} ->
   b1:bytes -> b2:bytes ->
   Lemma
-  (ensures get_label cusages (concat b1 b2) == meet (get_label cusages b1) (get_label cusages b2))
-  [SMTPat (get_label cusages (concat b1 b2))]
-let get_label_concat cusages b1 b2 =
+  (ensures get_label (concat b1 b2) == meet (get_label b1) (get_label b2))
+  [SMTPat (get_label (concat b1 b2))]
+let get_label_concat b1 b2 =
   normalize_term_spec concat;
   normalize_term_spec get_label
 
 val concat_preserves_knowability:
-  cinvs:crypto_invariants -> lab:label -> tr:trace ->
+  {|crypto_invariants|} -> lab:label -> tr:trace ->
   b1:bytes -> b2:bytes ->
   Lemma
-  (requires is_knowable_by cinvs lab tr b1 /\ is_knowable_by cinvs lab tr b2)
-  (ensures is_knowable_by cinvs lab tr (concat b1 b2))
-  [SMTPat (is_knowable_by cinvs lab tr (concat b1 b2))]
-let concat_preserves_knowability cinvs lab tr b1 b2 =
+  (requires is_knowable_by lab tr b1 /\ is_knowable_by lab tr b2)
+  (ensures is_knowable_by lab tr (concat b1 b2))
+  [SMTPat (is_knowable_by lab tr (concat b1 b2))]
+let concat_preserves_knowability #cinvs lab tr b1 b2 =
   normalize_term_spec concat;
   normalize_term_spec bytes_invariant;
   normalize_term_spec get_label
 
 val split_preserves_knowability:
-  cinvs:crypto_invariants -> lab:label -> tr:trace ->
+  {|crypto_invariants|} -> lab:label -> tr:trace ->
   b:bytes -> i:nat ->
   Lemma
-  (requires is_knowable_by cinvs lab tr b)
+  (requires is_knowable_by lab tr b)
   (ensures (
     match split b i with
     | None -> True
-    | Some (b1, b2) -> is_knowable_by cinvs lab tr b1 /\ is_knowable_by cinvs lab tr b2
+    | Some (b1, b2) -> is_knowable_by lab tr b1 /\ is_knowable_by lab tr b2
   ))
-let split_preserves_knowability cinvs lab tr b i =
+let split_preserves_knowability #cinvs lab tr b i =
   normalize_term_spec split;
   normalize_term_spec bytes_invariant;
   normalize_term_spec get_label
@@ -544,38 +554,38 @@ let aead_dec_enc key nonce msg ad =
 
 // Lemma for attacker knowledge theorem
 val aead_enc_preserves_publishability:
-  cinvs:crypto_invariants -> tr:trace ->
+  {|crypto_invariants|} -> tr:trace ->
   key:bytes -> nonce:bytes -> msg:bytes -> ad:bytes ->
   Lemma
   (requires
-    is_publishable cinvs tr key /\
-    is_publishable cinvs tr nonce /\
-    is_publishable cinvs tr msg /\
-    is_publishable cinvs tr ad
+    is_publishable tr key /\
+    is_publishable tr nonce /\
+    is_publishable tr msg /\
+    is_publishable tr ad
   )
-  (ensures is_publishable cinvs tr (aead_enc key nonce msg ad))
-let aead_enc_preserves_publishability cinvs tr key nonce msg ad =
+  (ensures is_publishable tr (aead_enc key nonce msg ad))
+let aead_enc_preserves_publishability #cinvs tr key nonce msg ad =
   normalize_term_spec aead_enc;
   normalize_term_spec bytes_invariant;
   normalize_term_spec get_label
 
 // Lemma for attacker knowledge theorem
 val aead_dec_preserves_publishability:
-  cinvs:crypto_invariants -> tr:trace ->
+  {|crypto_invariants|} -> tr:trace ->
   key:bytes -> nonce:bytes -> msg:bytes -> ad:bytes ->
   Lemma
   (requires
-    is_publishable cinvs tr key /\
-    is_publishable cinvs tr nonce /\
-    is_publishable cinvs tr msg /\
-    is_publishable cinvs tr ad
+    is_publishable tr key /\
+    is_publishable tr nonce /\
+    is_publishable tr msg /\
+    is_publishable tr ad
   )
   (ensures (
     match aead_dec key nonce msg ad with
-    | Some res -> is_publishable cinvs tr res
+    | Some res -> is_publishable tr res
     | None -> True
   ))
-let aead_dec_preserves_publishability cinvs tr key nonce msg ad =
+let aead_dec_preserves_publishability #cinvs tr key nonce msg ad =
   normalize_term_spec aead_dec;
   normalize_term_spec bytes_invariant;
   // F* needs the match for some reason?
@@ -584,64 +594,64 @@ let aead_dec_preserves_publishability cinvs tr key nonce msg ad =
   | None -> ()
 
 val bytes_invariant_aead_enc:
-  cinvs:crypto_invariants -> tr:trace ->
+  {|crypto_invariants|} -> tr:trace ->
   key:bytes -> nonce:bytes -> msg:bytes -> ad:bytes ->
   Lemma
   (requires
-    bytes_invariant cinvs tr key /\
-    bytes_invariant cinvs tr nonce /\
-    bytes_invariant cinvs tr msg /\
-    bytes_invariant cinvs tr ad /\
-    (get_label cinvs.usages nonce) `can_flow tr` public /\
-    (get_label cinvs.usages ad) `can_flow tr` public /\
-    (get_label cinvs.usages msg) `can_flow tr` (get_label cinvs.usages key) /\
-    AeadKey? (get_usage cinvs.usages key) /\
-    cinvs.preds.aead_pred tr key nonce msg ad
+    bytes_invariant tr key /\
+    bytes_invariant tr nonce /\
+    bytes_invariant tr msg /\
+    bytes_invariant tr ad /\
+    (get_label nonce) `can_flow tr` public /\
+    (get_label ad) `can_flow tr` public /\
+    (get_label msg) `can_flow tr` (get_label key) /\
+    AeadKey? (get_usage key) /\
+    aead_pred tr key nonce msg ad
   )
-  (ensures bytes_invariant cinvs tr (aead_enc key nonce msg ad))
-  [SMTPat (bytes_invariant cinvs tr (aead_enc key nonce msg ad))]
-let bytes_invariant_aead_enc cinvs tr key nonce msg ad =
+  (ensures bytes_invariant tr (aead_enc key nonce msg ad))
+  [SMTPat (bytes_invariant tr (aead_enc key nonce msg ad))]
+let bytes_invariant_aead_enc #cinvs tr key nonce msg ad =
   normalize_term_spec aead_enc;
   normalize_term_spec bytes_invariant
 
 val get_label_aead_enc:
-  cusages:crypto_usages ->
+  {|crypto_usages|} ->
   key:bytes -> nonce:bytes -> msg:bytes -> ad:bytes ->
   Lemma
-  (ensures get_label cusages (aead_enc key nonce msg ad) = public)
-  [SMTPat (get_label cusages (aead_enc key nonce msg ad))]
-let get_label_aead_enc cusages key nonce msg ad =
+  (ensures get_label (aead_enc key nonce msg ad) = public)
+  [SMTPat (get_label (aead_enc key nonce msg ad))]
+let get_label_aead_enc #cusages key nonce msg ad =
   normalize_term_spec aead_enc;
   normalize_term_spec get_label
 
 val bytes_invariant_aead_dec:
-  cinvs:crypto_invariants -> tr:trace ->
+  {|crypto_invariants|} -> tr:trace ->
   key:bytes -> nonce:bytes -> msg:bytes -> ad:bytes ->
   Lemma
   (requires
     // Actually only need the one on `msg`
-    bytes_invariant cinvs tr key /\
-    bytes_invariant cinvs tr nonce /\
-    bytes_invariant cinvs tr msg /\
-    bytes_invariant cinvs tr ad
+    bytes_invariant tr key /\
+    bytes_invariant tr nonce /\
+    bytes_invariant tr msg /\
+    bytes_invariant tr ad
   )
   (ensures (
     match aead_dec key nonce msg ad with
     | None -> True
     | Some plaintext -> (
-      is_knowable_by cinvs (get_label cinvs.usages key) tr plaintext /\
+      is_knowable_by (get_label key) tr plaintext /\
       (
         (
-          AeadKey? (get_usage cinvs.usages key) ==>
-          cinvs.preds.aead_pred tr key nonce plaintext ad
+          AeadKey? (get_usage key) ==>
+          aead_pred tr key nonce plaintext ad
         ) \/ (
-          is_publishable cinvs tr key
+          is_publishable tr key
         )
       )
     )
   ))
-  [SMTPat (aead_dec key nonce msg ad); SMTPat (bytes_invariant cinvs tr msg)]
-let bytes_invariant_aead_dec cinvs tr key nonce msg ad =
+  [SMTPat (aead_dec key nonce msg ad); SMTPat (bytes_invariant tr msg)]
+let bytes_invariant_aead_dec #cinvs tr key nonce msg ad =
   normalize_term_spec aead_dec;
   normalize_term_spec bytes_invariant;
   normalize_term_spec get_label;
@@ -683,146 +693,146 @@ let pk_dec_enc key nonce msg =
 
 // Lemma for attacker knowledge theorem
 val pk_preserves_publishability:
-  cinvs:crypto_invariants -> tr:trace ->
+  {|crypto_invariants|} -> tr:trace ->
   sk:bytes ->
   Lemma
-  (requires is_publishable cinvs tr sk)
-  (ensures is_publishable cinvs tr (pk sk))
-let pk_preserves_publishability cinvs tr sk =
+  (requires is_publishable tr sk)
+  (ensures is_publishable tr (pk sk))
+let pk_preserves_publishability #cinvs tr sk =
   normalize_term_spec pk;
   normalize_term_spec bytes_invariant;
   normalize_term_spec get_label
 
 // Lemma for attacker knowledge theorem
 val pk_enc_preserves_publishability:
-  cinvs:crypto_invariants -> tr:trace ->
+  {|crypto_invariants|} -> tr:trace ->
   pk:bytes -> nonce:bytes -> msg:bytes ->
   Lemma
   (requires
-    is_publishable cinvs tr pk /\
-    is_publishable cinvs tr nonce /\
-    is_publishable cinvs tr msg
+    is_publishable tr pk /\
+    is_publishable tr nonce /\
+    is_publishable tr msg
   )
-  (ensures is_publishable cinvs tr (pk_enc pk nonce msg))
-let pk_enc_preserves_publishability cinvs tr pk nonce msg =
+  (ensures is_publishable tr (pk_enc pk nonce msg))
+let pk_enc_preserves_publishability #cinvs tr pk nonce msg =
   normalize_term_spec pk_enc;
   normalize_term_spec bytes_invariant;
   normalize_term_spec get_label
 
 // Lemma for attacker knowledge theorem
 val pk_dec_preserves_publishability:
-  cinvs:crypto_invariants -> tr:trace ->
+  {|crypto_invariants|} -> tr:trace ->
   sk:bytes -> msg:bytes ->
   Lemma
   (requires
-    is_publishable cinvs tr sk /\
-    is_publishable cinvs tr msg
+    is_publishable tr sk /\
+    is_publishable tr msg
   )
   (ensures (
     match pk_dec sk msg with
-    | Some res -> is_publishable cinvs tr res
+    | Some res -> is_publishable tr res
     | None -> True
   ))
-let pk_dec_preserves_publishability cinvs tr sk msg =
+let pk_dec_preserves_publishability #cinvs tr sk msg =
   normalize_term_spec pk_dec;
   normalize_term_spec get_sk_label;
   normalize_term_spec bytes_invariant;
   normalize_term_spec get_label
 
 val bytes_invariant_pk:
-  cinvs:crypto_invariants -> tr:trace ->
+  {|crypto_invariants|} -> tr:trace ->
   sk:bytes ->
   Lemma
-  (requires bytes_invariant cinvs tr sk)
-  (ensures bytes_invariant cinvs tr (pk sk))
-  [SMTPat (bytes_invariant cinvs tr (pk sk))]
-let bytes_invariant_pk cinvs tr sk =
+  (requires bytes_invariant tr sk)
+  (ensures bytes_invariant tr (pk sk))
+  [SMTPat (bytes_invariant tr (pk sk))]
+let bytes_invariant_pk #cinvs tr sk =
   normalize_term_spec pk;
   normalize_term_spec bytes_invariant
 
 val get_label_pk:
-  cusages:crypto_usages ->
+  {|crypto_usages|} ->
   sk:bytes ->
   Lemma
-  (ensures get_label cusages (pk sk) == public)
-  [SMTPat (get_label cusages (pk sk))]
-let get_label_pk cusages sk =
+  (ensures get_label (pk sk) == public)
+  [SMTPat (get_label (pk sk))]
+let get_label_pk #cusages sk =
   normalize_term_spec pk;
   normalize_term_spec get_label
 
 val get_sk_label_pk:
-  cusages:crypto_usages ->
+  {|crypto_usages|} ->
   sk:bytes ->
   Lemma
-  (ensures get_sk_label cusages (pk sk) == get_label cusages sk)
-  [SMTPat (get_sk_label cusages (pk sk))]
-let get_sk_label_pk cusages sk =
+  (ensures get_sk_label (pk sk) == get_label sk)
+  [SMTPat (get_sk_label (pk sk))]
+let get_sk_label_pk #cusages sk =
   normalize_term_spec pk;
   normalize_term_spec get_sk_label
 
 val get_sk_usage_pk:
-  cusages:crypto_usages ->
+  {|crypto_usages|} ->
   sk:bytes ->
   Lemma
-  (ensures get_sk_usage cusages (pk sk) == get_usage cusages sk)
-  [SMTPat (get_sk_usage cusages (pk sk))]
-let get_sk_usage_pk cusages sk =
+  (ensures get_sk_usage (pk sk) == get_usage sk)
+  [SMTPat (get_sk_usage (pk sk))]
+let get_sk_usage_pk #cusages sk =
   normalize_term_spec pk;
   normalize_term_spec get_sk_usage
 
 val bytes_invariant_pk_enc:
-  cinvs:crypto_invariants -> tr:trace ->
+  {|crypto_invariants|} -> tr:trace ->
   pk:bytes -> nonce:bytes -> msg:bytes ->
   Lemma
   (requires
-    bytes_invariant cinvs tr pk /\
-    bytes_invariant cinvs tr nonce /\
-    bytes_invariant cinvs tr msg /\
-    (get_label cinvs.usages msg) `can_flow tr` (get_sk_label cinvs.usages pk) /\
-    (get_label cinvs.usages msg) `can_flow tr` (get_label cinvs.usages nonce) /\
-    PkdecKey? (get_sk_usage cinvs.usages pk) /\
-    cinvs.preds.pkenc_pred tr pk msg
+    bytes_invariant tr pk /\
+    bytes_invariant tr nonce /\
+    bytes_invariant tr msg /\
+    (get_label msg) `can_flow tr` (get_sk_label pk) /\
+    (get_label msg) `can_flow tr` (get_label nonce) /\
+    PkdecKey? (get_sk_usage pk) /\
+    pkenc_pred tr pk msg
   )
-  (ensures bytes_invariant cinvs tr (pk_enc pk nonce msg))
-  [SMTPat (bytes_invariant cinvs tr (pk_enc pk nonce msg))]
-let bytes_invariant_pk_enc cinvs tr pk nonce msg =
+  (ensures bytes_invariant tr (pk_enc pk nonce msg))
+  [SMTPat (bytes_invariant tr (pk_enc pk nonce msg))]
+let bytes_invariant_pk_enc #cinvs tr pk nonce msg =
   normalize_term_spec pk_enc;
   normalize_term_spec bytes_invariant
 
 val get_label_pk_enc:
-  cusages:crypto_usages ->
+  {|crypto_usages|} ->
   pk:bytes -> nonce:bytes -> msg:bytes ->
   Lemma
-  (ensures get_label cusages (pk_enc pk nonce msg) == public)
-  [SMTPat (get_label cusages (pk_enc pk nonce msg))]
-let get_label_pk_enc cusages pk nonce msg =
+  (ensures get_label (pk_enc pk nonce msg) == public)
+  [SMTPat (get_label (pk_enc pk nonce msg))]
+let get_label_pk_enc #cusages pk nonce msg =
   normalize_term_spec pk_enc;
   normalize_term_spec get_label
 
 val bytes_invariant_pk_dec:
-  cinvs:crypto_invariants -> tr:trace ->
+  {|crypto_invariants|} -> tr:trace ->
   sk:bytes -> msg:bytes ->
   Lemma
   (requires
-    bytes_invariant cinvs tr sk /\
-    bytes_invariant cinvs tr msg
+    bytes_invariant tr sk /\
+    bytes_invariant tr msg
   )
   (ensures (
     match pk_dec sk msg with
     | None -> True
     | Some plaintext ->
-      is_knowable_by cinvs (get_label cinvs.usages sk) tr plaintext /\
+      is_knowable_by (get_label sk) tr plaintext /\
       (
         (
-          PkdecKey? (get_sk_usage cinvs.usages (pk sk)) ==>
-          cinvs.preds.pkenc_pred tr (pk sk) plaintext
+          PkdecKey? (get_sk_usage (pk sk)) ==>
+          pkenc_pred tr (pk sk) plaintext
         ) \/ (
-          is_publishable cinvs tr plaintext
+          is_publishable tr plaintext
         )
       )
   ))
-  [SMTPat (pk_dec sk msg); SMTPat (bytes_invariant cinvs tr msg)]
-let bytes_invariant_pk_dec cinvs tr sk msg =
+  [SMTPat (pk_dec sk msg); SMTPat (bytes_invariant tr msg)]
+let bytes_invariant_pk_dec #cinvs tr sk msg =
   normalize_term_spec pk_dec;
   normalize_term_spec pk;
   normalize_term_spec get_sk_label;
@@ -860,122 +870,122 @@ let verify_sign sk nonce msg =
 
 // Lemma for attacker knowledge theorem
 val vk_preserves_publishability:
-  cinvs:crypto_invariants -> tr:trace ->
+  {|crypto_invariants|} -> tr:trace ->
   sk:bytes ->
   Lemma
-  (requires is_publishable cinvs tr sk)
-  (ensures is_publishable cinvs tr (vk sk))
-let vk_preserves_publishability cinvs tr sk =
+  (requires is_publishable tr sk)
+  (ensures is_publishable tr (vk sk))
+let vk_preserves_publishability #cinvs tr sk =
   normalize_term_spec vk;
   normalize_term_spec bytes_invariant;
   normalize_term_spec get_label
 
 // Lemma for attacker knowledge theorem
 val sign_preserves_publishability:
-  cinvs:crypto_invariants -> tr:trace ->
+  {|crypto_invariants|} -> tr:trace ->
   sk:bytes -> nonce:bytes -> msg:bytes ->
   Lemma
   (requires
-    is_publishable cinvs tr sk /\
-    is_publishable cinvs tr nonce /\
-    is_publishable cinvs tr msg
+    is_publishable tr sk /\
+    is_publishable tr nonce /\
+    is_publishable tr msg
   )
-  (ensures is_publishable cinvs tr (sign sk nonce msg))
-let sign_preserves_publishability cinvs tr sk nonce msg =
+  (ensures is_publishable tr (sign sk nonce msg))
+let sign_preserves_publishability #cinvs tr sk nonce msg =
   normalize_term_spec sign;
   normalize_term_spec bytes_invariant;
   normalize_term_spec get_label
 
 val bytes_invariant_vk:
-  cinvs:crypto_invariants -> tr:trace ->
+  {|crypto_invariants|} -> tr:trace ->
   sk:bytes ->
   Lemma
-  (requires bytes_invariant cinvs tr sk)
-  (ensures bytes_invariant cinvs tr (pk sk))
-  [SMTPat (bytes_invariant cinvs tr (pk sk))]
-let bytes_invariant_vk cinvs tr sk =
+  (requires bytes_invariant tr sk)
+  (ensures bytes_invariant tr (pk sk))
+  [SMTPat (bytes_invariant tr (pk sk))]
+let bytes_invariant_vk #cinvs tr sk =
   normalize_term_spec vk;
   normalize_term_spec bytes_invariant
 
 val get_label_vk:
-  cusages:crypto_usages ->
+  {|crypto_usages|} ->
   sk:bytes ->
   Lemma
-  (ensures get_label cusages (vk sk) == public)
-  [SMTPat (get_label cusages (vk sk))]
-let get_label_vk cusages sk =
+  (ensures get_label (vk sk) == public)
+  [SMTPat (get_label (vk sk))]
+let get_label_vk #cusages sk =
   normalize_term_spec vk;
   normalize_term_spec get_label
 
 val get_signkey_label_vk:
-  cusages:crypto_usages ->
+  {|crypto_usages|} ->
   sk:bytes ->
   Lemma
-  (ensures get_signkey_label cusages (vk sk) == get_label cusages sk)
-  [SMTPat (get_signkey_label cusages (vk sk))]
-let get_signkey_label_vk cusages sk =
+  (ensures get_signkey_label (vk sk) == get_label sk)
+  [SMTPat (get_signkey_label (vk sk))]
+let get_signkey_label_vk #cusages sk =
   normalize_term_spec vk;
   normalize_term_spec get_signkey_label
 
 val get_signkey_usage_vk:
-  cusages:crypto_usages ->
+  {|crypto_usages|} ->
   sk:bytes ->
   Lemma
-  (ensures get_signkey_usage cusages (vk sk) == get_usage cusages sk)
-  [SMTPat (get_signkey_usage cusages (vk sk))]
-let get_signkey_usage_vk cusages sk =
+  (ensures get_signkey_usage (vk sk) == get_usage sk)
+  [SMTPat (get_signkey_usage (vk sk))]
+let get_signkey_usage_vk #cusages sk =
   normalize_term_spec vk;
   normalize_term_spec get_signkey_usage
 
 val bytes_invariant_sign:
-  cinvs:crypto_invariants -> tr:trace ->
+  {|crypto_invariants|} -> tr:trace ->
   sk:bytes -> nonce:bytes -> msg:bytes ->
   Lemma
   (requires
-    bytes_invariant cinvs tr sk /\
-    bytes_invariant cinvs tr nonce /\
-    bytes_invariant cinvs tr msg /\
-    bytes_invariant cinvs tr sk /\
-    SigKey? (get_usage cinvs.usages sk) /\
-    cinvs.preds.sign_pred tr (vk sk) msg
+    bytes_invariant tr sk /\
+    bytes_invariant tr nonce /\
+    bytes_invariant tr msg /\
+    bytes_invariant tr sk /\
+    SigKey? (get_usage sk) /\
+    sign_pred tr (vk sk) msg
   )
-  (ensures bytes_invariant cinvs tr (sign sk nonce msg))
-  [SMTPat (bytes_invariant cinvs tr (sign sk nonce msg))]
-let bytes_invariant_sign cinvs tr sk nonce msg =
+  (ensures bytes_invariant tr (sign sk nonce msg))
+  [SMTPat (bytes_invariant tr (sign sk nonce msg))]
+let bytes_invariant_sign #cinvs tr sk nonce msg =
   normalize_term_spec sign;
   normalize_term_spec vk;
   normalize_term_spec bytes_invariant
 
 val get_label_sign:
-  cusages:crypto_usages ->
+  {|crypto_usages|} ->
   sk:bytes -> nonce:bytes -> msg:bytes ->
   Lemma
-  (ensures get_label cusages (sign sk nonce msg) == get_label cusages msg)
-  [SMTPat (get_label cusages (sign sk nonce msg))]
-let get_label_sign cusages sk nonce msg =
+  (ensures get_label (sign sk nonce msg) == get_label msg)
+  [SMTPat (get_label (sign sk nonce msg))]
+let get_label_sign #cusages sk nonce msg =
   normalize_term_spec sign;
   normalize_term_spec get_label
 
 val bytes_invariant_verify:
-  cinvs:crypto_invariants -> tr:trace ->
+  {|crypto_invariants|} -> tr:trace ->
   vk:bytes -> msg:bytes -> signature:bytes ->
   Lemma
   (requires
-    bytes_invariant cinvs tr vk /\
-    bytes_invariant cinvs tr msg /\
-    bytes_invariant cinvs tr signature /\
+    bytes_invariant tr vk /\
+    bytes_invariant tr msg /\
+    bytes_invariant tr signature /\
     verify vk msg signature
   )
   (ensures
     (
-      SigKey? (get_signkey_usage cinvs.usages vk) ==>
-      cinvs.preds.sign_pred tr vk msg
+      SigKey? (get_signkey_usage vk) ==>
+      sign_pred tr vk msg
     ) \/ (
-      (get_signkey_label cinvs.usages vk) `can_flow tr` public
+      (get_signkey_label vk) `can_flow tr` public
     )
   )
-  [SMTPat (verify vk msg signature); SMTPat (bytes_invariant cinvs tr signature)]
-let bytes_invariant_verify cinvs tr vk msg signature =
+  [SMTPat (verify vk msg signature); SMTPat (bytes_invariant tr signature)]
+let bytes_invariant_verify #cinvs tr vk msg signature =
   normalize_term_spec verify;
   normalize_term_spec get_signkey_label;
   normalize_term_spec bytes_invariant;
@@ -989,34 +999,34 @@ let hash msg = Hash msg
 
 // Lemma for attacker knowledge theorem
 val hash_preserves_publishability:
-  cinvs:crypto_invariants -> tr:trace ->
+  {|crypto_invariants|} -> tr:trace ->
   msg:bytes ->
   Lemma
-  (requires is_publishable cinvs tr msg)
-  (ensures is_publishable cinvs tr (hash msg))
-let hash_preserves_publishability cinvs tr msg =
+  (requires is_publishable tr msg)
+  (ensures is_publishable tr (hash msg))
+let hash_preserves_publishability #cinvs tr msg =
   normalize_term_spec hash;
   normalize_term_spec bytes_invariant;
   normalize_term_spec get_label
 
 // Lemmas for the user
 val bytes_invariant_hash:
-  cinvs:crypto_invariants -> tr:trace ->
+  {|crypto_invariants|} -> tr:trace ->
   msg:bytes ->
   Lemma
-  (requires bytes_invariant cinvs tr msg)
-  (ensures bytes_invariant cinvs tr (hash msg))
-  [SMTPat (hash msg); SMTPat (bytes_invariant cinvs tr msg)]
-let bytes_invariant_hash cinvs tr msg =
+  (requires bytes_invariant tr msg)
+  (ensures bytes_invariant tr (hash msg))
+  [SMTPat (hash msg); SMTPat (bytes_invariant tr msg)]
+let bytes_invariant_hash #cinvs tr msg =
   normalize_term_spec hash;
   normalize_term_spec bytes_invariant
 
 val get_label_hash:
-  cusages:crypto_usages ->
+  {|crypto_usages|} ->
   msg:bytes ->
-  Lemma (get_label cusages (hash msg) == get_label cusages msg)
-  [SMTPat (get_label cusages (hash msg))]
-let get_label_hash cusages msg =
+  Lemma (get_label (hash msg) == get_label msg)
+  [SMTPat (get_label (hash msg))]
+let get_label_hash #cusages msg =
   normalize_term_spec hash;
   normalize_term_spec get_label
 
