src/DY.Core.Attacker.Knowledge.fst
@@ -111,63 +111,63 @@ let move_requires_4 #a #b #c #d #p #q pf x y z w =
   introduce p x y z w ==> q x y z w with _. pf x y z w
 
 val corrupted_state_is_publishable:
-  invs:protocol_invariants ->
+  {|protocol_invariants|} ->
   tr:trace -> prin:principal -> sess_id:nat -> content:bytes ->
   Lemma
   (requires
     principal_state_corrupt tr prin sess_id /\
     state_was_set tr prin sess_id content /\
-    trace_invariant invs tr
+    trace_invariant tr
   )
-  (ensures is_publishable invs.crypto_invs tr content)
-let corrupted_state_is_publishable invs tr prin sess_id content =
-  state_is_knowable_by invs tr prin sess_id content
+  (ensures is_publishable tr content)
+let corrupted_state_is_publishable #invs tr prin sess_id content =
+  state_is_knowable_by tr prin sess_id content
 
 #push-options "--z3rlimit 25"
 val attacker_only_knows_publishable_values_aux:
-  invs:protocol_invariants ->
+  {|protocol_invariants|} ->
   step:nat -> tr:trace -> msg:bytes ->
   Lemma
   (requires
-    trace_invariant invs tr /\
+    trace_invariant tr /\
     attacker_knows_aux step tr msg
   )
-  (ensures is_publishable invs.crypto_invs tr msg)
-let rec attacker_only_knows_publishable_values_aux invs step tr msg =
+  (ensures is_publishable tr msg)
+let rec attacker_only_knows_publishable_values_aux #invs step tr msg =
   if step = 0 then (
-    FStar.Classical.forall_intro   (FStar.Classical.move_requires   (msg_sent_on_network_are_publishable invs tr));
-    FStar.Classical.forall_intro   (FStar.Classical.move_requires   (msg_sent_on_network_are_publishable invs tr));
-    FStar.Classical.forall_intro_3 (FStar.Classical.move_requires_3 (corrupted_state_is_publishable invs tr));
-    FStar.Classical.forall_intro   (FStar.Classical.move_requires   (literal_to_bytes_is_publishable invs.crypto_invs tr))
+    FStar.Classical.forall_intro   (FStar.Classical.move_requires   (msg_sent_on_network_are_publishable tr));
+    FStar.Classical.forall_intro   (FStar.Classical.move_requires   (msg_sent_on_network_are_publishable tr));
+    FStar.Classical.forall_intro_3 (FStar.Classical.move_requires_3 (corrupted_state_is_publishable tr));
+    FStar.Classical.forall_intro   (FStar.Classical.move_requires   (literal_to_bytes_is_publishable tr))
   ) else (
-    FStar.Classical.forall_intro   (FStar.Classical.move_requires   (attacker_only_knows_publishable_values_aux invs (step-1) tr));
-    FStar.Classical.forall_intro_2 (FStar.Classical.move_requires_2 (concat_preserves_publishability invs.crypto_invs tr));
-    FStar.Classical.forall_intro_2 (FStar.Classical.move_requires_2 (split_preserves_publishability invs.crypto_invs tr));
-    FStar.Classical.forall_intro_4 (                move_requires_4 (aead_enc_preserves_publishability invs.crypto_invs tr));
-    FStar.Classical.forall_intro_4 (                move_requires_4 (aead_dec_preserves_publishability invs.crypto_invs tr));
-    FStar.Classical.forall_intro   (FStar.Classical.move_requires   (pk_preserves_publishability invs.crypto_invs tr));
-    FStar.Classical.forall_intro_3 (FStar.Classical.move_requires_3 (pk_enc_preserves_publishability invs.crypto_invs tr));
-    FStar.Classical.forall_intro_2 (FStar.Classical.move_requires_2 (pk_dec_preserves_publishability invs.crypto_invs tr));
-    FStar.Classical.forall_intro   (FStar.Classical.move_requires   (vk_preserves_publishability invs.crypto_invs tr));
-    FStar.Classical.forall_intro_3 (FStar.Classical.move_requires_3 (sign_preserves_publishability invs.crypto_invs tr));
-    FStar.Classical.forall_intro   (FStar.Classical.move_requires   (hash_preserves_publishability invs.crypto_invs tr));
+    FStar.Classical.forall_intro   (FStar.Classical.move_requires   (attacker_only_knows_publishable_values_aux (step-1) tr));
+    FStar.Classical.forall_intro_2 (FStar.Classical.move_requires_2 (concat_preserves_publishability tr));
+    FStar.Classical.forall_intro_2 (FStar.Classical.move_requires_2 (split_preserves_publishability tr));
+    FStar.Classical.forall_intro_4 (                move_requires_4 (aead_enc_preserves_publishability tr));
+    FStar.Classical.forall_intro_4 (                move_requires_4 (aead_dec_preserves_publishability tr));
+    FStar.Classical.forall_intro   (FStar.Classical.move_requires   (pk_preserves_publishability tr));
+    FStar.Classical.forall_intro_3 (FStar.Classical.move_requires_3 (pk_enc_preserves_publishability tr));
+    FStar.Classical.forall_intro_2 (FStar.Classical.move_requires_2 (pk_dec_preserves_publishability tr));
+    FStar.Classical.forall_intro   (FStar.Classical.move_requires   (vk_preserves_publishability tr));
+    FStar.Classical.forall_intro_3 (FStar.Classical.move_requires_3 (sign_preserves_publishability tr));
+    FStar.Classical.forall_intro   (FStar.Classical.move_requires   (hash_preserves_publishability tr));
     ()
   )
 #pop-options
 
 val attacker_only_knows_publishable_values:
-  invs:protocol_invariants ->
+  {|protocol_invariants|} ->
   tr:trace -> msg:bytes ->
   Lemma
   (requires
-    trace_invariant invs tr /\
+    trace_invariant tr /\
     attacker_knows tr msg
   )
-  (ensures is_publishable invs.crypto_invs tr msg)
-let attacker_only_knows_publishable_values invs tr msg =
+  (ensures is_publishable tr msg)
+let attacker_only_knows_publishable_values #invs tr msg =
   reveal_opaque (`%attacker_knows) (attacker_knows);
   eliminate exists step. attacker_knows_aux step tr msg
-  returns is_publishable invs.crypto_invs tr msg
+  returns is_publishable tr msg
   with _. (
-    attacker_only_knows_publishable_values_aux invs step tr msg
+    attacker_only_knows_publishable_values_aux step tr msg
   )
